BreadBoard/Common.v
@@ -1,0 +1,11 @@
+
+Fixpoint len {T:Type}(x : list T) : nat :=
+  match x with
+    | x::b => 1+len b
+    | nil => 0
+  end.
+Fixpoint suml (x : list nat) : nat :=
+  match x with
+    | x::b => x+suml b
+    | nil => 0
+  end.
