BreadBoard/Component.v
@@ -1,0 +1,10 @@
+
+Import IO.
+Module Type Component_Sig(IO:IO_SIG).
+  Variable io : IO.func.
+End Component_Sig.
+
+Module Component(I:IO_SIG)(M:Component_Sig(I)).
+  Import M.
+  Definition io := M.io.
+End Component.
