BreadBoard/IO.v
@@ -1,0 +1,19 @@
+
+Module Type IO_SIG.
+  Variable t : Type.
+  Variable trace : Set.
+  Variable func : Set.
+  Variable nargs : func -> nat.
+End IO_SIG.
+
+Module IO.
+  Definition t :=  nat.
+  Definition trace := list (list t).
+  Inductive func_ :=
+  | fn_args : nat -> (trace -> t) -> func_.
+  Definition func := func_.
+  Definition nargs f :=
+    match f with
+      | fn_args n _ => n
+    end.
+End IO.
