BreadBoard/Run.v
@@ -1,0 +1,63 @@
+
+Module IORUN.
+
+
+  Definition pin_trace_gen w : list (nat* list IO.t):= map (fun p => (p, nil)) (pins w).
+  Search option.
+  Fixpoint find_trace p pt  : option (list IO.t) :=
+    match pt with 
+      | [] => None
+      | (p', t)::rest => if beq_nat p' p then Some t else find_trace p rest 
+    end.
+  Definition find_traces (p :list nat) (pt : list (nat * list IO.t))  : option (list (list IO.t)) :=
+    let elts :=map (fun f =>  (find_trace f pt))  p in
+    let none := forallb (fun x => match x with | None => false | _ => true end ) elts in
+    if none then 
+      Some (map (fun f =>  match f with | None => [] | Some x => x end) elts)
+    else None.
+
+  Definition any_trace  (pt : list (nat * list IO.t) ): list IO.t :=
+    match pt with 
+      | nil => nil
+      | (p', t)::rest => t
+    end.
+  Fixpoint update_trace pt u acc:=
+    match u with
+      | (p, iot)::rest =>
+        match find_trace p pt with
+          | None => update_trace pt rest acc
+          | Some trace =>
+            update_trace pt rest ((p, iot::trace)::acc)
+        end
+      | [] => acc
+    end.
+  Print IO.func.
+  Fixpoint step' w pt (u : list (nat * IO.t))  :=
+    let add_i := set_add in 
+    match w with 
+      | base  =>
+        update_trace pt (u) nil
+      | watch_set w' from (IO.fn_args n fn) to =>
+        let o_traces := (find_traces from pt) in
+        match o_traces with
+          | None => pt
+          | Some traces =>
+            step' w' pt ((to, fn traces )::u)
+        end
+      |  just_set w' (IO.fn_args n fn) to =>
+         step' w' pt  ((to, fn [any_trace  pt ])::u)
+      | join w1 w2 =>
+        app (step' w2 pt [])  (step' w1 pt u)
+      | doc w' _ _ => step' w' pt u
+    end.
+  Definition step w :=
+    step' w (pin_trace_gen w) [].
+
+  Fixpoint run' (w:wiring) (pt: list (nat * list IO.t)) fuel  :=
+    match fuel with
+      | O => pt
+      | S n => run' w (step' w pt []) n
+    end.
+  Definition run w fuel :=
+    run' w (pin_trace_gen w) fuel.
+End IORUN.
