BreadBoard/Wiring.v
@@ -1,0 +1,137 @@
+Module Wiring(IO:IO_SIG).
+  Inductive wiring :=
+  | base :  wiring
+  | watch_set :  wiring -> list nat -> IO.func -> nat ->  wiring
+  | just_set : wiring  -> IO.func -> nat -> wiring
+  | join : wiring -> wiring -> wiring
+  | doc : wiring -> nat -> string -> wiring.
+  Notation  "w //  m ~> f ~>  n" := (watch_set w m f n) (at level 80, m at next level). 
+  Notation  "w */  f ~>  n" := (just_set w f n) (at level 80, m at next level). 
+  Notation "w1 ~&~ w2" := (join w1 w2) (at level 80).
+  Notation "w # p c " := (doc w p c) (at level 80, p at level 0).
+
+  Open Scope string_scope.
+  Fixpoint docstring' w acc :=
+    match w with
+      | base  => acc
+      | watch_set w' from fn to => docstring' w' acc
+      | just_set w' fn to =>docstring' w' acc
+      | join w1 w2 => docstring' w2 (docstring' w1 acc)
+      | doc w' p c =>
+        let n : string := (String (ascii_of_nat p) "") in 
+        docstring' w' ("Port" ++ n ++ c ++ "\n" ++ acc)
+
+    end.
+  Definition docstring w := docstring' w "".
+  Fixpoint output_pins w s: set nat :=
+    let add_i := set_add%nat nat eq_nat_dec in
+    match w with 
+      | base  =>
+        s
+      | watch_set w' from fn to =>
+        output_pins w' (add_i  to s)
+      | just_set w' fn to =>
+        output_pins w' (add_i to s)
+      | join w1 w2 => set_union%nat nat eq_nat_dec (output_pins w1 s) (output_pins w2 nil)
+      | doc w' _ _ =>  output_pins w' s
+    end.
+
+  Fixpoint input_pins w s: set nat :=
+    let add_i := set_add%nat nat eq_nat_dec in
+    match w with 
+      | base  => s
+      | watch_set w' from fn to =>
+        output_pins w'
+                    (fold_left (fun se f => add_i f se) s  from)
+
+      | just_set w' fn to =>  output_pins w' s
+      | join w1 w2 => set_union%nat nat eq_nat_dec (output_pins w1 s) (output_pins w2 nil)
+      | doc w' _ _ =>  input_pins w' s
+    end.
+
+  Fixpoint all_pins' w s: set nat :=
+    let add_i := set_add%nat nat eq_nat_dec in
+    match w with 
+      | base  => s
+      | watch_set w' from fn to =>
+        all_pins' w'
+                  (add_i to (fold_left (fun se f => add_i f se) s  from))
+
+      | just_set w' fn to =>  all_pins' w' (add_i to s)
+      | join w1 w2 => set_union%nat nat eq_nat_dec (all_pins' w1 s) (all_pins' w2 nil)
+      | doc w' _ _ =>  all_pins' w' s
+    end.
+  Definition pins w := all_pins' w nil.
+  (* Checks that all observers have a source and that only one setter per nat *)
+  Fixpoint valid_wiring' w ins outs: Prop :=
+    let add_i := set_add%nat nat eq_nat_dec in
+    let notin := (fun el  s => (not (set_In%nat nat  el s))) in
+    let union := set_union%nat nat eq_nat_dec in
+    let intersect := set_inter%nat nat eq_nat_dec in
+    match w with 
+      | base  =>
+        (* Check that the intersection of inputs and outputs is inputs,
+         ie, everything can be read *)
+        (intersect ins outs) = ins
+      | watch_set w' from fn to =>
+        notin to outs /\
+        IO.nargs fn = length from /\
+        valid_wiring' w'
+                      ( fold_left  (fun s f => add_i f s) ins from) (add_i to outs)
+      | just_set w' fn to=>
+        notin to outs
+        /\ valid_wiring' w' ins (add_i to outs)
+      | join w1 w2 =>
+        let w1_out := output_pins w1 [] in
+        let w2_out := output_pins w2 [] in
+        (* intersect w1_out w2_out = [] /\ (*is implicitly checked*)  *) 
+        (* We union in the others outputs to say that w2 is promising
+        that it will make this available as an output (so treat it as an
+        available input too *)
+        valid_wiring' w1 (union w2_out ins) (union
+                                               w2_out outs) /\
+        valid_wiring' w2  (union w1_out ins) (union w1_out outs)
+      | doc w' _ _ =>  valid_wiring' w'  ins outs
+    end.
+  Definition valid_wiring w : Prop :=
+    valid_wiring' w nil nil.
+
+  Require Import Omega.
+  Ltac autowire :=
+    unfold valid_wiring;
+    unfold valid_wiring';
+    simpl;
+    repeat (try split; try omega).
+
+  (* Rewire w1 so it won't interfere with w2 *)
+  Fixpoint rewire_offset w1 n: wiring :=
+    match w1 with
+      | base => base
+      | watch_set w' from fn to =>
+         (watch_set  (rewire_offset w' n) (map (fun x=>x+ n)from) fn (to+n))
+      | just_set w' fn to =>
+      just_set  (rewire_offset w' n) fn (to+n) 
+      | join w1 w2 =>
+        join (rewire_offset w1 n) ( rewire_offset w2 n ) 
+      | doc w' p c =>  
+         (doc  (rewire_offset w' n ) (p+n) c)
+    end.
+  Definition rewire w1 w2 : wiring :=
+    let m := fold_left max (pins w2) 0 in
+    rewire_offset w1 m.
+
+  Theorem rewire_safe : forall w w',
+                          valid_wiring w ->
+                          valid_wiring w' ->
+                          valid_wiring (rewire w w' ~&~ w').
+    intros.
+    unfold valid_wiring.
+    unfold valid_wiring'.
+    simpl.
+    fold valid_wiring'.
+    fold valid_wiring.
+    split.
+    admit.
+    admit.
+  Qed.
+End Wiring.
